theories/Dot/typing/typing_unstamped_derived.v
@@ -2,6 +2,7 @@ From stdpp Require Import strings.
 From D Require Import tactics.
 From D.Dot Require Import syn synLemmas exampleInfra typing_unstamped.
 From D.Dot Require Import unstampedness_binding.
+From D.Dot Require Import path_repl_lemmas typingStamping.
 Import DBNotation.
 
 Lemma is_unstamped_pvar i n : i < n → is_unstamped_path n (pv (var_vl i)).
@@ -10,6 +11,15 @@ Hint Resolve is_unstamped_pvar : core.
 Lemma is_unstamped_pvars i n l : i < n → is_unstamped_ty n (pv (var_vl i) @; l).
 Proof. eauto. Qed.
 Hint Resolve is_unstamped_pvars : core.
+Lemma unstamped_subject_closed {Γ e T}
+  (Ht : Γ u⊢ₜ e : T) :
+  nclosed e (length Γ).
+Proof.
+  destruct (stamp_objIdent_typed Ht ∅); ev. exact: is_unstamped_nclosed_tm.
+Qed.
+
+Lemma var_typed_closed {Γ x T} : Γ u⊢ₜ tv (ids x) : T → x < length Γ.
+Proof. by move => /unstamped_subject_closed/fv_of_val_inv/nclosed_var_lt. Qed.
 
 Ltac typconstructor := match goal with
   | |- typed _ _ _ => constructor
@@ -21,6 +31,43 @@ Ltac typconstructor := match goal with
 
 (* Ltac tcrush := repeat first [ fast_done | typconstructor | stcrush ]. *)
 Ltac tcrush := repeat first [ eassumption | reflexivity | typconstructor | stcrush ].
+
+Lemma Appv_typed Γ e1 x2 T1 T2:
+  Γ u⊢ₜ e1: TAll T1 T2 →
+  Γ u⊢ₜ tv (var_vl x2) : T1 →
+  is_unstamped_ty (S (length Γ)) T2 →
+  (*────────────────────────────────────────────────────────────*)
+  Γ u⊢ₜ tapp e1 (tv (var_vl x2)) : T2.|[(var_vl x2)/].
+Proof.
+  intros He1 Hx2 Hu. have Hlx2 := var_typed_closed Hx2.
+  rewrite -(psubst_subst_agree_ty (n := S (length Γ))); tcrush.
+  eapply App_path_typed with (p2 := (pv (var_vl x2))); tcrush.
+Qed.
+
+Lemma TMuE_typed Γ x T:
+  Γ u⊢ₜ tv (var_vl x): TMu T →
+  (*──────────────────────*)
+  is_unstamped_ty (S (length Γ)) T →
+  Γ u⊢ₜ tv (var_vl x): T.|[(var_vl x)/].
+Proof.
+  move => + Hu. rewrite -(psubst_subst_agree_ty (n := S (length Γ))) // => Hx.
+  by apply (Path_typed (p := pv (ids x))), p_mu_e_typed, pv_typed, Hx.
+Qed.
+
+Lemma TMuI_typed Γ x T:
+  Γ u⊢ₜ tv (var_vl x): T.|[(var_vl x)/] →
+  (*──────────────────────*)
+  is_unstamped_ty (S (length Γ)) T →
+  Γ u⊢ₜ tv (var_vl x): TMu T.
+Proof.
+  move => + Hu. rewrite -(psubst_subst_agree_ty (n := S (length Γ))) // => Hx.
+  by apply (Path_typed (p := pv (ids x))), p_mu_i_typed, pv_typed, Hx.
+Qed.
+
+Ltac tcrush ::=
+  repeat first [ eassumption | reflexivity |
+  apply TMuI_typed | apply TMuE_typed |
+  typconstructor | stcrush ].
 
 Lemma is_unstamped_TLater_n i {n T}:
   is_unstamped_ty n T →
@@ -121,16 +168,18 @@ Ltac varsub := (eapply Var0_typed_sub || eapply Var_typed_sub); first done.
 Lemma Appv_typed' T2 {Γ e1 x2 T1 T3} :
   Γ u⊢ₜ e1: TAll T1 T2 →                        Γ u⊢ₜ tv (ids x2) : T1 →
   T3 = T2.|[ids x2/] →
+  is_unstamped_ty (S (length Γ)) T2 →
   (*────────────────────────────────────────────────────────────*)
   Γ u⊢ₜ tapp e1 (tv (ids x2)) : T3.
-Proof. intros; subst; by econstructor. Qed.
+Proof. intros; subst; exact: Appv_typed. Qed.
 
 Lemma TMuE_typed' Γ x T1 T2:
   Γ u⊢ₜ tv (ids x): μ T1 →
   T2 = T1.|[ids x/] →
+  is_unstamped_ty (S (length Γ)) T1 →
   (*──────────────────────*)
   Γ u⊢ₜ tv (ids x): T2.
-Proof. intros; subst; auto. Qed.
+Proof. intros; subst; tcrush. Qed.
 
 Lemma Sub_later_shift {Γ T1 T2 i j}
   (Hs1: is_unstamped_ty (length Γ) T1)
@@ -359,7 +408,7 @@ Lemma tyApp_typed Γ T U V t l :
   Γ u⊢ₜ tyApp t l T : V.
 Proof.
   move => Ht Hsub HuT1 HuU1.
-  eapply Let_typed; [exact: Ht| |tcrush].
+  eapply Let_typed; [exact: Ht| |wtcrush].
   eapply Let_typed; [apply packTV_typed| |]; wtcrush.
   rewrite /= -!hrenS -/(typeEq _ _).
 
@@ -369,6 +418,9 @@ Proof.
   have HuT3 : is_unstamped_ty (S (S (length Γ))) (shiftN 2 T)
     by rewrite hrenS; wtcrush.
   varsub; tcrush; rewrite !hsubst_comp; f_equal. autosubst.
+  asimpl.
+  eapply is_unstamped_sub_ren_ty, HuU1.
+  by move => [|i] Hi //=; [constructor => /=| eauto].
 Qed.
 
 (** * Manipulating laters, more.
@@ -580,47 +632,3 @@ Lemma AnfBind_typed Γ t (T U: ty) :
   is_unstamped_ty (length Γ) T →
   Γ u⊢ₜ anfBind t : U.
 Proof. intros; eapply Let_typed; eauto. Qed.
-
-From D.Dot Require Import path_repl_lemmas typingStamping.
-
-Lemma unstamped_subject_closed {Γ e T}
-  (Ht : Γ u⊢ₜ e : T) :
-  nclosed e (length Γ).
-Proof.
-  destruct (stamp_objIdent_typed Ht ∅); ev. exact: is_unstamped_nclosed_tm.
-Qed.
-
-Lemma var_typed_closed {Γ x T} : Γ u⊢ₜ tv (ids x) : T → x < length Γ.
-Proof. by move => /unstamped_subject_closed/fv_of_val_inv/nclosed_var_lt. Qed.
-
-Lemma Appv_typed_derived Γ e1 x2 T1 T2:
-  Γ u⊢ₜ e1: TAll T1 T2 →
-  Γ u⊢ₜ tv (var_vl x2) : T1 →
-  is_unstamped_ty (S (length Γ)) T2 →
-  (*────────────────────────────────────────────────────────────*)
-  Γ u⊢ₜ tapp e1 (tv (var_vl x2)) : T2.|[(var_vl x2)/].
-Proof.
-  intros He1 Hx2 Hu. have Hlx2 := var_typed_closed Hx2.
-  rewrite -(psubst_subst_agree_ty (n := S (length Γ))); tcrush.
-  eapply App_path_typed with (p2 := (pv (var_vl x2))); tcrush.
-Qed.
-
-Lemma TMuE_typed_derived Γ x T:
-  Γ u⊢ₜ tv (var_vl x): TMu T →
-  (*──────────────────────*)
-  is_unstamped_ty (S (length Γ)) T →
-  Γ u⊢ₜ tv (var_vl x): T.|[(var_vl x)/].
-Proof.
-  move => + Hu. rewrite -(psubst_subst_agree_ty (n := S (length Γ))) // => Hx.
-  by apply (Path_typed (p := pv (ids x))), p_mu_e_typed, pv_typed, Hx.
-Qed.
-
-Lemma TMuI_typed_derived Γ x T:
-  Γ u⊢ₜ tv (var_vl x): T.|[(var_vl x)/] →
-  (*──────────────────────*)
-  is_unstamped_ty (S (length Γ)) T →
-  Γ u⊢ₜ tv (var_vl x): TMu T.
-Proof.
-  move => + Hu. rewrite -(psubst_subst_agree_ty (n := S (length Γ))) // => Hx.
-  by apply (Path_typed (p := pv (ids x))), p_mu_i_typed, pv_typed, Hx.
-Qed.
